x86/AsmregsC.v
@@ -1,0 +1,175 @@
+Require Import CoqlibC Maps.
+Require Import Values.
+Require Import Locations Stacklayout Conventions.
+Require Import MemoryC Integers AST.
+(** newly added **)
+Require Export Asmregs.
+Require Import Locations.
+
+
+Module PLAYGROUND.
+(* Lemma extcall_arguments_perm_aux *)
+(*       rs m tys vs *)
+(*       ir fr (* ofs *) *)
+(*       (ARGS: list_forall2 (extcall_arg_pair rs m) (loc_arguments_64 tys ir fr 0) vs) *)
+(*       sp spofs *)
+(*       (RSPPTR: rs RSP = Vptr sp spofs true) *)
+(*   : *)
+(*     <<PERM: Mem.range_perm m sp (Ptrofs.unsigned spofs) *)
+(*                            (Ptrofs.unsigned spofs + size_arguments_64 tys ir fr 0) Cur Nonempty>> *)
+(* . *)
+(* Proof. *)
+(*   ginduction tys; i. *)
+(*   { ii. inv ARGS. ss. xomega. } *)
+(*   destruct a; inv ARGS; try (by des_ifs). *)
+(*   - specialize (IHtys _ _ _ _ _ H1). *)
+(* Qed. *)
+
+
+
+
+(* Lemma loc_arguments_64_complete *)
+(*       x tys ir fr *)
+(*       (SIZE0: x < 4 * size_arguments_64 tys ir fr 0) *)
+(*       (SIZE1: 0 <= x) *)
+(*       (IR: 0 <= ir) *)
+(*       (FR: 0 <= fr) *)
+(*   : *)
+(*     exists sl pos ty, <<IN: In (S sl pos ty) (loc_arguments_64 tys ir fr 0).(regs_of_rpairs)>> *)
+(*                             /\ <<OFS: pos <= x < pos + 4 * ty.(typesize)>> *)
+(* . *)
+(* Proof. *)
+(*   ginduction tys; ii; ss. *)
+(*   { xomega. } *)
+(*   destruct a; ss. *)
+(*   - des. *)
+(*     des_ifs; try (exploit IHtys; eauto; try xomega; i; des; []; esplits; eauto; ss; right; eauto). *)
+(*     assert(6 <= ir). *)
+(*     { xomega. } *)
+(*     ss. esplits; eauto; try xomega. ss. rewrite Z.add_0_l in *. rewrite Z.mul_1_r. *)
+(*     unfold size_arguments_64 in SIZE0. ss. des_ifs. *)
+(*     u in SIZE0. *)
+(*     destruct ir; try xomega. *)
+(*     ss. *)
+(*   - *)
+(* Qed. *)
+Lemma typesize_chunk
+      ty
+  :
+    4 * ty.(typesize) = size_chunk (chunk_of_type ty)
+.
+Proof. destruct ty; ss. Qed.
+
+Print extcall_arg.
+Local Opaque Z.mul Z.add Z.div Z.sub.
+Local Opaque list_nth_z.
+Lemma size_arguments_loc_arguments
+      ofs
+      tys ir fr acc
+      (SIZE: acc <= ofs < size_arguments_64 tys ir fr acc)
+  :
+    exists pos ty, <<IN: In (S Outgoing pos ty) (loc_arguments_64 tys ir fr acc).(regs_of_rpairs)>> /\
+                            <<BOUND: pos <= ofs < pos + ty.(typesize)>>
+.
+Proof.
+  unfold size_arguments in *. unfold loc_arguments in *.
+  ginduction tys; ii; ss.
+  { xomega. }
+  destruct a; ss.
+  - des_ifs.
+    + exploit IHtys; eauto. i; des. esplits; cbn; eauto.
+    + cbn.
+      do 2 eexists. split; eauto. red. ss.
+      admit "IT DOES NOT HOLD!!!!!!!!!!!!!!!!!!!!!!!!!!!!!!!!!!!!!!!!!! 2 ofs for int value !!!!!!!!!!!!".
+  - admit "".
+  - admit "".
+  - admit "".
+  - admit "".
+  - admit "".
+Qed.
+
+Lemma extcall_arguments_perm_aux
+      rs m tys vs
+      ir fr (* ofs *)
+      (ARGS: list_forall2 (extcall_arg_pair rs m) (loc_arguments_64 tys ir fr 0) vs)
+      sp
+      (RSPPTR: rs RSP = Vptr sp Ptrofs.zero true)
+  :
+    <<PERM: Mem.range_perm m sp 0 (4 * (size_arguments_64 tys ir fr 0)) Cur Nonempty>>
+.
+Proof.
+  assert(BOUND: forall
+            loc
+            (IN: In loc (loc_arguments_64 tys ir fr 0))
+          ,
+            exists v, In v vs /\ extcall_arg_pair rs m loc v).
+  { ii. eapply list_forall2_in_left; eauto. }
+
+  ii.
+  set (ofsdiv := ofs/4).
+  assert(DIVBOUND: 0 <= ofsdiv < size_arguments_64 tys ir fr 0).
+  { admit "". }
+  exploit size_arguments_loc_arguments; eauto. i; des.
+  assert(POS: 0 <= pos).
+  { admit "easy". }
+  exploit in_regs_of_rpairs_inv; eauto. i; des.
+  exploit BOUND; eauto. i; des.
+  inv H4.
+  - Local Opaque Z.mul.
+    inv H5; ss; des; clarify.
+    unfold fe_ofs_arg in *.
+    rewrite RSPPTR in *.
+    ss. rewrite Ptrofs.add_zero_l in *. rewrite Z.add_0_l in *.
+    (* rewrite Ptrofs.unsigned_repr in *; cycle 1. *)
+    (* { *)
+    exploit Mem.load_valid_access; eauto. intro VALID; des. hnf in VALID. des.
+    eapply Mem.perm_implies with (p1 := Readable); [|eauto with mem].
+    eapply VALID. rewrite <- typesize_chunk.
+    split.
+    + rewrite Ptrofs.unsigned_repr_eq.
+      assert(4 * pos <= ofs).
+      { admit "". }
+      etransitivity; eauto. eapply Z.mod_le; try xomega.
+      generalize Ptrofs.modulus_pos. i. xomega.
+    + assert(ofs < 4 * pos + 4 * (typesize ty)).
+      { admit "". }
+      rewrite Ptrofs.unsigned_repr_eq. eapply Z.lt_le_trans; eauto.
+      apply Z.add_le_mono_r.
+      admit "somehow..".
+  - admit "".
+Qed.
+
+Lemma extcall_arguments_perm
+      rs m sg vs
+      (ARGS: extcall_arguments rs m sg vs)
+      sp
+      (RSPPTR: (rs RSP) = Vptr sp Ptrofs.zero true)
+  :
+    Mem.range_perm m sp 0 (size_arguments sg) Cur Nonempty
+.
+Proof.
+(*   unfold extcall_arguments in *. *)
+(*   destruct sg; ss. unfold loc_arguments, size_arguments in *. ss. des_ifs. clear_tac. *)
+(*   ginduction sig_args; i; ss. *)
+(*   { ii. xomega. } *)
+(*   destruct a; ss. *)
+(*   - inv ARGS. *)
+(* Qed. *)
+Admitted.
+
+
+End PLAYGROUND.
+
+(* Reset size_arguments_loc_arguments. *)
+
+
+Inductive load_arguments (rs_arg: regset) (m_arg: mem) (sg_init: signature)
+          (vs_init: list val) (m_init: mem): Prop :=
+| load_arguments_intro
+    sp
+    (RSPPTR: rs_arg RSP = Vptr sp Ptrofs.zero true)
+    (PERM: Mem.range_perm m_arg sp 0 (size_arguments sg_init) Cur Nonempty)
+    (VAL: extcall_arguments rs_arg m_arg sg_init vs_init)
+    (DROP: Mem_set_perm m_arg sp 0 (4 * (size_arguments sg_init)) None = Some m_init)
+.
+
